src/proofs/no_slashable_attestations/supporting_lemmas/ind_inv_implies_safety/core_proofs.dfy
@@ -54,7 +54,7 @@ module Core_Proofs
     requires inv_sent_validity_predicate_only_for_slots_stored_in_att_slashing_db_hist(dv)
     requires inv_all_validity_predicates_are_stored_in_att_slashing_db_hist(dv)
     requires inv_sent_validity_predicate_is_based_on_rcvd_duty_and_slashing_db_in_hist(dv)
-    requires inv_sent_validity_predicate_is_based_on_rcvd_duty_and_slashing_db_in_histii(dv)
+    requires inv_db_of_validity_predicate_contains_all_previous_decided_values(dv)
     requires inv_queued_att_duty_is_rcvd_duty0(dv)
     // requires inv_queued_att_duty_is_rcvd_duty1(dv)
     ensures && !is_slashable_attestation_data_eth_spec(a.data, a'.data)
@@ -175,7 +175,7 @@ module Core_Proofs
     requires pred_data_of_att_share_is_decided_value(dv)
     requires inv_decided_value_of_consensus_instance_is_decided_by_quorum(dv)    
     requires inv_sent_validity_predicate_is_based_on_rcvd_duty_and_slashing_db_in_hist(dv)
-    requires inv_sent_validity_predicate_is_based_on_rcvd_duty_and_slashing_db_in_histii(dv)
+    requires inv_db_of_validity_predicate_contains_all_previous_decided_values(dv)
     requires && a in dv.all_attestations_created
              && is_valid_attestation(a, dv.dv_pubkey)
     requires && a' in dv.all_attestations_created
@@ -213,7 +213,7 @@ module Core_Proofs
     requires pred_data_of_att_share_is_decided_value(dv)
     requires inv_decided_value_of_consensus_instance_is_decided_by_quorum(dv)    
     requires inv_sent_validity_predicate_is_based_on_rcvd_duty_and_slashing_db_in_hist(dv)
-    requires inv_sent_validity_predicate_is_based_on_rcvd_duty_and_slashing_db_in_histii(dv)
+    requires inv_db_of_validity_predicate_contains_all_previous_decided_values(dv)
     requires && a in dv.all_attestations_created
              && is_valid_attestation(a, dv.dv_pubkey)
     requires && a' in dv.all_attestations_created
@@ -257,7 +257,7 @@ module Core_Proofs
     requires pred_data_of_att_share_is_decided_value(dv)
     requires inv_decided_value_of_consensus_instance_is_decided_by_quorum(dv)    
     requires inv_sent_validity_predicate_is_based_on_rcvd_duty_and_slashing_db_in_hist(dv)
-    requires inv_sent_validity_predicate_is_based_on_rcvd_duty_and_slashing_db_in_histii(dv)
+    requires inv_db_of_validity_predicate_contains_all_previous_decided_values(dv)
     requires && a in dv.all_attestations_created
              && is_valid_attestation(a, dv.dv_pubkey)
     requires && a' in dv.all_attestations_created
